cava/arrow-examples/Aes/cipher_round.v
@@ -1,0 +1,52 @@
+(****************************************************************************)
+(* Copyright 2020 The Project Oak Authors                                   *)
+(*                                                                          *)
+(* Licensed under the Apache License, Version 2.0 (the "License")           *)
+(* you may not use this file except in compliance with the License.         *)
+(* You may obtain a copy of the License at                                  *)
+(*                                                                          *)
+(*     http://www.apache.org/licenses/LICENSE-2.0                           *)
+(*                                                                          *)
+(* Unless required by applicable law or agreed to in writing, software      *)
+(* distributed under the License is distributed on an "AS IS" BASIS,        *)
+(* WITHOUT WARRANTIES OR CONDITIONS OF ANY KIND, either express or implied. *)
+(* See the License for the specific language governing permissions and      *)
+(* limitations under the License.                                           *)
+(****************************************************************************)
+
+From Coq Require Import Arith Eqdep_dec Vector Lia NArith Omega String Ndigits.
+From Arrow Require Import Category Arrow.
+From Cava Require Import Arrow.ArrowExport BitArithmetic.
+
+From ArrowExamples Require Import Combinators Aes.pkg Aes.mix_columns Aes.sbox Aes.sub_bytes Aes.shift_rows.
+
+Import VectorNotations.
+Import KappaNotation.
+Open Scope kind_scope.
+
+Definition cipher_round
+  (sbox_impl: SboxImpl)
+  : << Bit                               (* cipher mode: CIPH_FWD/CIPH_INV *)
+    , Vector (Vector (Vector Bit 8) 4) 4 (* data input *)
+    , Vector (Vector (Vector Bit 8) 4) 4 (* round key *)
+    , Unit>> ~>
+      Vector (Vector (Vector Bit 8) 4) 4 :=
+  <[\op_i data_i key =>
+    let stage1 = !(aes_sub_bytes sbox_impl) op_i data_i in
+    let stage2 = !aes_shift_rows op_i stage1 in
+    let stage3 = !aes_mix_columns op_i stage2 in
+    stage3 ^ key
+    ]>.
+
+Definition final_cipher_round
+  (sbox_impl: SboxImpl)
+  : << Bit                               (* cipher mode: CIPH_FWD/CIPH_INV *)
+    , Vector (Vector (Vector Bit 8) 4) 4 (* data input *)
+    , Vector (Vector (Vector Bit 8) 4) 4 (* round key *)
+    , Unit>> ~>
+      Vector (Vector (Vector Bit 8) 4) 4 :=
+  <[\op_i data_i key =>
+    let stage1 = !(aes_sub_bytes sbox_impl) op_i data_i in
+    let stage2 = !aes_shift_rows op_i stage1 in
+    stage2 ^ key
+    ]>.
